progress on Reification tactics

reify/reverse_reify.v
@@ -5,8 +5,11 @@ Require Import progs.reverse.
 Require Import progs.list_dt.
 Require Import sep.
 Require Import wrapExpr.
+Require Import MirrorShard.ReifySepExpr.
+Require Import MirrorShard.ReifyExpr.
 Local Open Scope logic.
 
+Unset Ltac Debug.
 
 (*Some definitions needed from the example file (verif_reverse.v) *)
 Instance LS: listspec t_struct_list _tail.
@@ -273,12 +276,14 @@ Definition list_spec_tv := Expr.tvType (length our_types).
 
 (*Separation logic predicate just for this file *)
 
-Definition lseg_signature :=
+Definition lseg_LS := lseg LS.
+
+Definition lseg_LS_signature :=
 Sep.PSig all_types (cons share_tv
                    (cons list_val_tv (cons val_tv (cons val_tv nil))))
-(lseg LS).
+(lseg_LS).
 
-Definition predicates := (lseg_signature :: nil).
+Definition predicates := (lseg_LS_signature :: nil).
 Definition lseg_p := length sep_predicates.
 
 
@@ -324,6 +329,184 @@ Definition sum_int_func i1  :=
 Definition i_func := nullary_func i_f.
 Definition cts_func := nullary_func cts_f.
 Definition y_func := nullary_func y_f.
+
+(*Tactics for reifying derives and hypothesis *)
+
+Lemma convert_inj : forall S Q, !!S && Q  = (!!S && emp) * Q.
+intros.
+apply pred_ext.
+ entailer!. 
+entailer!.
+Qed.
+
+(*When prepare_reify is finished, all !!s should be in the form
+!!P && emp * ... so that they can be converted to SepExpr.Inj 
+this tactic is likely incomplete*)
+
+Ltac fold_seplog := 
+fold VericSepLogic_Kernel.star VericSepLogic.star
+VericSepLogic_Kernel.emp VericSepLogic.emp
+VericSepLogic_Kernel.inj VericSepLogic.inj
+VericSepLogic_Kernel.ex VericSepLogic.ex.
+
+Ltac prepare_reify :=
+autorewrite with gather_prop;
+match goal with 
+| [ |- !!?X && _ |-- !!?Y && _] => rewrite (convert_inj X); rewrite (convert_inj Y)
+| [ |- !!?X && _ |-- _] => rewrite (convert_inj X)
+| [ |- _ |-- _] => idtac
+end;
+fold_seplog.
+
+(*Turns a reified derives into a reified goal with no assumptions, 
+sort of a base case for rev_reify *)
+Ltac start_goalD :=
+match goal with 
+[ |- derivesD ?t ?f ?p ?e ?v ?d] => 
+replace (derivesD t f p e v d) with (goalD t f p e v (nil, d)) by reflexivity
+end.
+
+(*Pulls down any reified assumptions and puts them into 
+a goal *)
+
+Ltac rev_reify :=
+repeat match goal with
+| [ H : force_Opt (Expr.exprD ?f ?e ?v ?P ?ty) False |- goalD ?t ?f ?p ?e ?v (?l, ?d) ] => revert H; 
+replace (force_Opt (Expr.exprD f e v P ty) False ->
+goalD t f p e v (l, d)) with
+(goalD t f p e v (P::l, d)) by reflexivity
+end.
+
+Ltac abbreviate_goal :=
+match goal with
+[ |- goalD _ ?f ?p ?u _ _] => 
+abbreviate f as funcs;
+abbreviate p as preds;
+abbreviate u as uenv
+end.
+
+
+Ltac finish_reify :=
+match goal with 
+[ |- @Sep.sexprD ?t ?f ?p ?e ?v ?le |-- Sep.sexprD ?f ?p ?e ?v ?re ] => 
+  replace (Sep.sexprD f p e v le |-- Sep.sexprD f p e v re) with 
+  (derivesD t f p e v (le, re)) by reflexivity end;
+start_goalD;
+rev_reify;
+abbreviate_goal.
+
+Ltac get_types :=
+match goal with 
+| [ H := ?X : (list Expr.type) |- _] => X
+end.
+
+Ltac clear_types :=
+match goal with 
+| [ H := ?X : (list Expr.type) |- _] => unfold H in *; clear H
+end.
+
+Ltac get_funcs t := 
+match goal with
+[ _ := ?X : list (Expr.signature t) |- _ ] => X end.
+
+Ltac get_predicates t :=
+match goal with
+[ _ := ?X : list (Sep.predicate t) |- _] => X end.
+
+Ltac get_uenv t := 
+match goal with 
+| [ _ := ?X : Expr.env t |- _ ] => X
+| [ _ := ?X : list (sigT (Expr.tvarD t)) |- _ ] => X
+| [ _ : _ |- _ ] => constr:(@nil (sigT (Expr.tvarD all_types)))
+end.
+
+Ltac replace_reify_e H v r :=
+let types := get_types in
+let funcs := get_funcs types in
+let uenv := get_uenv types in
+replace v with 
+(force_Opt (@Expr.exprD types funcs uenv nil r Expr.tvProp)False) in H; [ | try reflexivity]. 
+
+Ltac reflect_sexpr types evars :=
+let reflect_sexpr' uvars funcs sfuncs s :=
+constr:(Sep.sexprD types funcs sfuncs uvars evars s) in
+reflect_sexpr'.
+
+Ltac reify_assumption H r:=
+match goal with
+[ H : ?X |- _] => replace_reify_e H X r
+end.
+
+Ltac replace_reify_s e r :=
+let types := get_types in
+let funcs := get_funcs types in
+let preds := get_predicates types in 
+let uenv := get_uenv types in 
+replace e with
+(@Sep.sexprD types funcs preds uenv  nil r); [ | try reflexivity ].
+
+Ltac replace_reify_s2 e funcs preds uenv r :=
+let types := get_types in
+replace e with
+(@Sep.sexprD types funcs preds uenv  nil r); [ | try reflexivity ].
+
+Module ReifySepM := ReifySepExpr VericSepLogic Sep.
+
+Ltac reify_derives :=
+prepare_reify;
+let types := get_types in
+let funcs := get_funcs types in
+let preds := get_predicates types in 
+let uenv := get_uenv types in
+match goal with
+[ |- ?ls |-- ?rs ] => 
+ReifySepM.reify_sexpr is_const ls types funcs tt tt
+preds uenv nil 
+ltac:(fun uenv' funcs' preds' ls_r => 
+ReifySepM.reify_sexpr is_const rs types funcs' tt tt
+preds' uenv' nil ltac:(fun uenv'' funcs'' preds'' rs_r =>
+replace_reify_s2 ls funcs'' preds'' uenv'' ls_r;
+replace_reify_s2 rs funcs'' preds'' uenv'' rs_r)) 
+end;
+try finish_reify.
+
+(*Tests for reifier*)
+(*Note: The continuation k must return a TACTIC to be executed on completion, not a value*)
+
+Ltac is_const e := 
+match type of e with
+| type => constr:(true)
+| ident => constr:(true)
+| _ => 
+  match e with 
+  | nil => constr:(true)
+  | nullval => constr:(true)
+  | _ => constr:(false)
+  end
+end.
+
+Ltac id_this ex := assert (forall n, ex = n).
+
+Lemma test_reify_expr : forall (rho:environ),
+False. 
+Proof.
+intros.
+reify_expr is_const (typed_true (tptr t_struct_list) (eval_id _t rho)) all_types functions
+0 0  ltac:(fun a b c => id_this c).
+Admitted.
+
+Lemma test_reify_sexpr : forall (rho:environ) (contents : list int) (sh : share),
+lseg_LS sh nil (eval_id _p rho) nullval * emp |-- emp.
+Proof.
+intros.
+pose (types := all_types).
+pose (funcs := functions).
+pose (predicates := predicates).
+reify_derives.
+simpl.
+Check goalD.
+abbreviate_goal.
+Admitted.
 
 (*Some constants we will use *)
 
@@ -382,97 +565,6 @@ tc_environ_func delta_c rho_func.
 
 Ltac unfold_VericSepLogic := simpl; unfold VericSepLogic.star, 
 VericSepLogic.inj, VericSepLogic.emp.
-
-Lemma convert_inj : forall S Q, !!S && Q  = (!!S && emp) * Q.
-intros.
-apply pred_ext.
- entailer!. 
-entailer!.
-Qed.
-
-(*When prepare_reify is finished, all !!s should be in the form
-!!P && emp * ... so that they can be converted to SepExpr.Inj 
-this tactic is likely incomplete*)
-Ltac prepare_reify :=
-autorewrite with gather_prop;
-match goal with 
-| [ |- !!?X && _ |-- !!?Y && _] => rewrite (convert_inj X); rewrite (convert_inj Y)
-| [ |- !!?X && _ |-- _] => rewrite (convert_inj X)
-end.
-
-(*Turns a reified derives into a reified goal with no assumptions, 
-sort of a base case for rev_reify *)
-Ltac start_goalD :=
-match goal with 
-[ |- derivesD ?t ?f ?p ?e ?v ?d] => 
-replace (derivesD t f p e v d) with (goalD t f p e v (nil, d)) by reflexivity
-end.
-
-(*Pulls down any reified assumptions and puts them into 
-a goal *)
-Ltac rev_reify :=
-repeat match goal with
-| [ H : force_Opt (Expr.exprD ?f ?e ?v ?P ?ty) False |- goalD ?t ?f ?p ?e ?v (?l, ?d) ] => revert H; 
-replace (force_Opt (Expr.exprD f e v P ty) False ->
-goalD t f p e v (l, d)) with
-(goalD t f p e v (P::l, d)) by reflexivity
-end.
-
-Ltac finish_reify :=
-match goal with 
-[ |- @Sep.sexprD ?t ?f ?p ?e ?v ?le |-- Sep.sexprD ?f ?p ?e ?v ?re ] => 
-  replace (Sep.sexprD f p e v le |-- Sep.sexprD f p e v re) with 
-  (derivesD t f p e v (le, re)) by reflexivity end;
-start_goalD;
-rev_reify.
-
-Ltac get_types :=
-match goal with 
-| [ H := ?X : (list Expr.type) |- _] => X
-end.
-
-Ltac get_funcs t := 
-match goal with
-[ _ := ?X : list (Expr.signature t) |- _ ] => X end.
-
-Ltac get_predicates t :=
-match goal with
-[ _ := ?X : list (Sep.predicate t) |- _] => X end.
-
-Ltac get_uenv t := 
-match goal with 
-| [ _ := ?X : Expr.env t |- _ ] => X
-| [ _ := ?X : list (sigT (Expr.tvarD t)) |- _ ] => X
-| [ _ : _ |- _ ] => constr:(@nil (sigT (Expr.tvarD all_types)))
-end.
-
-Ltac replace_reify_e H v r :=
-let types := get_types in
-let funcs := get_funcs types in
-let uenv := get_uenv types in
-replace v with 
-(force_Opt (@Expr.exprD types funcs uenv nil r Expr.tvProp)False) in H; [ | try reflexivity]. 
-
-Ltac reify_assumption H r:=
-match goal with
-[ H : ?X |- _] => replace_reify_e H X r
-end.
-
-Ltac replace_reify_s e r :=
-let types := get_types in
-let funcs := get_funcs types in
-let preds := get_predicates types in 
-let uenv := get_uenv types in 
-replace e with
-(@Sep.sexprD types funcs preds uenv  nil r); [ | try reflexivity ].
-
-Ltac reify_derives l r :=
-prepare_reify;
-match goal with
-[ |- ?ls |-- ?rs ] => 
-replace_reify_s ls l; replace_reify_s rs r
-end;
-try finish_reify.
 
 
 Lemma while_entail1 :
