reify/wrapExpr.v
@@ -1,0 +1,35 @@
+Require Import sep.
+Require Import MirrorShard.Expr.
+Require Import floyd.proofauto.
+
+Definition assumptions types := list (Expr.expr types).
+Definition derives_r types := prod (Sep.sexpr types) (Sep.sexpr types).
+Definition goal types := prod (assumptions types) (derives_r types).
+
+Definition force_Opt {T} p (d:T) :=
+match p with
+| Some p' => p'
+| None => d
+end.
+
+Fixpoint assumptionsD types functions meta_env var_env assumptions :=
+match assumptions with 
+| cons h nil => force_Opt (@Expr.exprD types functions meta_env var_env h tvProp) True 
+| cons h t => force_Opt (@Expr.exprD types functions meta_env var_env h tvProp) True -> assumptionsD types functions meta_env var_env t
+| nil => True
+end.
+
+Definition derivesD types functions preds meta_env var_env (der : derives_r types) :=
+let (l,r) := der in
+@Sep.sexprD types functions preds meta_env var_env l
+|--
+@Sep.sexprD types functions preds meta_env var_env r. 
+
+Fixpoint goalD types functions preds meta_env var_env (goal : goal types) :=
+let (assumptions, derives) := goal in
+match assumptions with 
+| nil => derivesD types functions preds meta_env var_env derives
+| _ => 
+assumptionsD types functions meta_env var_env assumptions ->
+derivesD types functions preds meta_env var_env derives
+end.
